tests/lean/run/nary_existsi.lean
@@ -1,0 +1,6 @@
+example : ∃ a b c : nat, a = b + c :=
+begin
+  existsi [_, _, _],
+  refl,
+  repeat {exact 0}
+end
